Lang/Typing.v
@@ -1,55 +1,582 @@
 Require Import Utf8.
-Require Import Binding.Lib Binding.Product Binding.Env.
+Require Import Binding.Lib Binding.Product Binding.Env Binding.Set.
 Require Import Syntax.
+Require Import String.
 
 Local Open Scope bind_scope.
 
 Inductive ttype :=
+  (* propositional atom *)
+  | tp_atom   : string → ttype
   | tp_bottom : ttype
   | tp_arrow  : ttype → ttype → ttype.
 Inductive ktype :=
   (* type of a continuation (A → ⊥⊥) *)
   | tp_cont   : ttype → ktype.
 
-Definition envV A := A → ttype.
-Definition envK A := A → ktype.
+Record env (A : VSig) := {
+  env_v : tv A → ttype;
+  env_k : kv A → ktype
+}.
 
-(* We use two environments:
-   Δ for continuation variables and Γ for term variables *)
-Reserved Notation "'T[' Δ ';' Γ '⊢' M '∷' A ']'".
-Reserved Notation "'J[' Δ ';' Γ '⊢' J '∷' '⊥⊥' ']'".
+Arguments env_v {A}.
+Arguments env_k {A}.
 
-Inductive ttyping {V K : Set} (Δ : envK K) (Γ : envV V) : term ⟨V, K⟩ → ttype → Prop :=
-  | T_Var : ∀ x,
-    T[ Δ; Γ ⊢ v_var x ∷ Γ x ]
+Definition empty_env := {|
+  env_v := λ (x : tv ⟨∅, ∅⟩), match x with end;
+  env_k := λ k, match k with end;
+|}.
+
+Definition extend_v {S : VSig} Γ A := {|
+  env_v := extend (env_v Γ) A : tv (incV S) → ttype;
+  env_k := env_k Γ
+|}.
+Notation "Γ '↦ᵥ' A" := (extend_v Γ A) (at level 67).
+
+Definition extend_k {S : VSig} (Γ : env S) K := {|
+  env_v := env_v Γ : tv (incK S) → ttype;
+  env_k := extend (env_k Γ) K;
+|}.
+Notation "Γ '↦ₖ' K" := (extend_k Γ K) (at level 67).
+
+(* Typing judgement for continuation atoms:
+   A is the type M needs to be for q M to be a jump. *)
+Reserved Notation "'K[' Γ '⊢' q '∷' A '→⊥⊥' ']'".
+Inductive ktyping {S : VSig} (Γ : env S) : katom S → ttype → Prop :=
+  | K_Tp :
+    (* ------------------- *)
+    K[ Γ ⊢ k_tp ∷ tp_bottom →⊥⊥ ]
+
+  | K_Var : ∀ k A,
+    env_k Γ k = tp_cont A →
+    (* -------------- *)
+    K[ Γ ⊢ k_var k ∷ A →⊥⊥ ]
+
+where "K[ Γ ⊢ q ∷ A →⊥⊥ ]" := (@ktyping _ Γ q A).
+
+Reserved Notation "'T[' Γ '⊢' M '∷' A  ']'".
+Reserved Notation "'J[' Γ '⊢' J '∷' '⊥⊥'  ']'".
+
+Inductive ttyping {S : VSig} (Γ : env S) : term S → ttype → Prop :=
+  | T_Var : ∀ x A,
+    env_v Γ x = A →
+    (* -------------- *)
+    T[ Γ ⊢ v_var x ∷ A ]
 
   | T_App : ∀ M N A B,
-    T[ Δ; Γ ⊢ M ∷ tp_arrow A B ] →
-    T[ Δ; Γ ⊢ N ∷ A ] →
-    (* --------------------*)
-    T[ Δ; Γ ⊢ t_app M N ∷ B ]
+    T[ Γ ⊢ M ∷ tp_arrow A B ] →
+    T[ Γ ⊢ N ∷ A ] →
+    (* ---------------- *)
+    T[ Γ ⊢ t_app M N ∷ B ]
 
   | T_Abs : ∀ M A B,
-    T[ Δ; Γ▹A ⊢ M ∷ B ] →
-    (* ---------------------------- *)
-    T[ Δ; Γ ⊢ v_lam M ∷ tp_arrow A B ]
+    T[ Γ ↦ᵥ A ⊢ M ∷ B ] →
+    (* ------------------------- *)
+    T[ Γ ⊢ v_lam M ∷ tp_arrow A B ]
 
   | T_Ctrl : ∀ J A,
-    J[ Δ▹tp_cont A; Γ ⊢ J ∷ ⊥⊥ ] →
-    (* ------------------ *)
-    T[ Δ; Γ ⊢ t_ctrl J ∷ A ]
+    J[ Γ ↦ₖ tp_cont A ⊢ J ∷ ⊥⊥ ] →
+    (* --------------- *)
+    T[ Γ ⊢ t_ctrl J ∷ A ]
 
-with jtyping {V K : Set} (Δ : envK K) (Γ : envV V) : jump ⟨V, K⟩ → Prop :=
+with jtyping {S : VSig} (Γ : env S) : jump S → Prop :=
   | J_Tp : ∀ M,
-    T[ Δ; Γ ⊢ M ∷ tp_bottom ] →
-    (* ----------------------- *)
-    J[ Δ; Γ ⊢ j_jmp k_tp M ∷ ⊥⊥ ]
+    T[ Γ ⊢ M ∷ tp_bottom ] →
+    (* -------------------- *)
+    J[ Γ ⊢ j_jmp k_tp M ∷ ⊥⊥ ]
 
   | J_Cont : ∀ M A k,
-    Δ k = tp_cont A →
-    T[ Δ; Γ ⊢ M ∷ A ] →
-    (* ---------------------------- *)
-    J[ Δ; Γ ⊢ j_jmp (k_var k) M ∷ ⊥⊥ ]
+    K[ Γ ⊢ k_var k ∷ A →⊥⊥ ] →
+    T[ Γ ⊢ M ∷ A ] →
+    (* ------------------------- *)
+    J[ Γ ⊢ j_jmp (k_var k) M ∷ ⊥⊥ ]
 
-where "T[ Δ ; Γ ⊢ M ∷ A ]"  := (@ttyping _ _ Δ Γ M A)
-  and "J[ Δ ; Γ ⊢ J ∷ ⊥⊥ ]" := (@jtyping _ _ Δ Γ J).
+where "T[ Γ ⊢ M ∷ A ]"  := (@ttyping _ Γ M A)
+  and "J[ Γ ⊢ J ∷ ⊥⊥ ]" := (@jtyping _ Γ J).
+
+(* Typing judgement for evaluation contexts:
+   E will have type A after plugging a term of type B. *)
+Reserved Notation "'E[' Γ '⊢' E '∷' A '⇐' B  ']'".
+Inductive etyping {S : VSig} (Γ : env S) : ectx S → ttype → ttype → Prop :=
+  | E_Hole : ∀ A,
+    (* ----------------- *)
+    E[ Γ ⊢ e_hole ∷ A ⇐ A ]
+
+  | E_AppL : ∀ E M A B U,
+    E[ Γ ⊢ E ∷ tp_arrow A B ⇐ U ] →
+    T[ Γ ⊢ M ∷ A ] →
+    (* --------------------- *)
+    E[ Γ ⊢ e_appl E M ∷ B ⇐ U ]
+
+  | E_AppR : ∀ E (V : value S) A B U,
+    T[ Γ ⊢ V ∷ tp_arrow A B ] →
+    E[ Γ ⊢ E ∷ A ⇐ U ] →
+    (* --------------------- *)
+    E[ Γ ⊢ e_appr V E ∷ B ⇐ U ]
+
+where "E[ Γ ⊢ E ∷ A ⇐ B ]" := (@etyping _ Γ E A B).
+
+Lemma etyping_correct {S : VSig} (Γ : env S) E M A B :
+  E[ Γ ⊢ E ∷ A ⇐ B ] →
+  T[ Γ ⊢ M ∷ B ] →
+  T[ Γ ⊢ eplug E M ∷ A ].
+Proof.
+  intros HE HM.
+  induction HE.
+  + simpl. apply HM.
+  + simpl. econstructor.
+    - apply IHHE. apply HM.
+    - apply H.
+  + simpl. econstructor.
+    - apply H.
+    - apply IHHE. apply HM.
+Qed.
+
+(* ========================================================================= *)
+(* fmap, weakening lemmas *)
+
+(* φ is a renaming that preserves types between Γ and Δ. *)
+Definition env_map_equiv {A B : VSig} (φ : @prod_arr _ _ Arr Arr A B) (Γ : env A) (Δ : env B) :=
+  (∀ x, env_v Δ (arr₁ φ x) = env_v Γ x)
+  ∧ (∀ k, env_k Δ (arr₂ φ k) = env_k Γ k).
+
+Lemma env_map_equiv_tv_extend {S T : VSig} (φ : prod_arr S T) Γ Δ A :
+  env_map_equiv φ Γ Δ → env_map_equiv (φ ↑) (Γ ↦ᵥ A) (Δ ↦ᵥ A).
+Proof.
+  intro Hφ.
+  split.
+  - destruct x as [| x].
+    * simpl. reflexivity.
+    * simpl. apply Hφ.
+  - intros k. simpl. apply Hφ.
+Qed.
+
+Lemma env_map_equiv_kv_extend {S T : VSig} (φ : prod_arr S T) Γ Δ A :
+  env_map_equiv φ Γ Δ → env_map_equiv (φ ↑) (Γ ↦ₖ A) (Δ ↦ₖ A).
+Proof.
+  intro Hφ.
+  split.
+  - intro x. simpl. apply Hφ.
+  - destruct k as [| k].
+    * simpl. reflexivity.
+    * simpl. apply Hφ.
+Qed.
+
+(* --------------------------------- *)
+
+Lemma ktyping_fmap {S T : VSig} (φ : prod_arr S T) (Γ : env S) (Δ : env T) q A :
+  env_map_equiv φ Γ Δ →
+  K[ Γ ⊢ q ∷ A →⊥⊥ ] → K[ Δ ⊢ fmap φ q ∷ A →⊥⊥ ].
+Proof.
+  intros Hφ Hq.
+  destruct Hq.
+  + constructor.
+  + constructor. rewrite (proj2 Hφ). apply H.
+Qed.
+
+Lemma ktyping_fmap2 {S T : VSig} (φ : prod_arr S T) (Γ : env S) (Δ : env T) q A :
+  env_map_equiv φ Γ Δ →
+  K[ Δ ⊢ fmap φ q ∷ A →⊥⊥ ] → K[ Γ ⊢ q ∷ A →⊥⊥ ].
+Proof.
+  intros Hφ Hq.
+  destruct q.
+  + inversion Hq as [| ? ? Hk ]; subst.
+    constructor. rewrite <- (proj2 Hφ). apply Hk.
+  + inversion Hq; subst.
+    constructor.
+Qed.
+
+Lemma ktyping_tv_weaken {S : VSig} (Γ : env S) (q : katom S) A B :
+  K[ Γ ⊢ q ∷ A →⊥⊥ ] ↔ K[ Γ ↦ᵥ B ⊢ shift q ∷ A →⊥⊥ ].
+Proof.
+  split.
+  + apply ktyping_fmap. split; reflexivity.
+  + apply ktyping_fmap2. split; reflexivity.
+Qed.
+
+Lemma ktyping_kv_weaken {S : VSig} (Γ : env S) (q : katom S) A B :
+  K[ Γ ⊢ q ∷ A →⊥⊥ ] ↔ K[ Γ ↦ₖ B ⊢ shift q ∷ A →⊥⊥ ].
+Proof.
+  split.
+  + apply ktyping_fmap. split; reflexivity.
+  + apply ktyping_fmap2. split; reflexivity.
+Qed.
+
+(* --------------------------------- *)
+
+Lemma ttyping_fmap {S T : VSig} (φ : prod_arr S T) (Γ : env S) (Δ : env T) M A :
+  env_map_equiv φ Γ Δ →
+  T[ Γ ⊢ M ∷ A ] → T[ Δ ⊢ fmap φ M ∷ A ]
+with jtyping_fmap {S T : VSig} (φ : prod_arr S T) (Γ : env S) (Δ : env T) J :
+  env_map_equiv φ Γ Δ →
+  J[ Γ ⊢ J ∷ ⊥⊥ ] → J[ Δ ⊢ fmap φ J ∷ ⊥⊥ ].
+Proof.
+(* ttyping_fmap *)
+{
+  intros Hφ HM.
+  generalize dependent Δ.
+  generalize dependent T.
+  induction HM; intros T φ Δ Hφ.
+  + term_simpl. constructor. subst. apply Hφ.
+  + term_simpl. econstructor.
+    - apply IHHM1. apply Hφ.
+    - apply IHHM2. apply Hφ.
+  + term_simpl. constructor.
+    apply IHHM. simpl. unfold env_map_equiv. split.
+    - destruct x.
+      * simpl. reflexivity.
+      * simpl. apply Hφ.
+    - intro k. simpl. apply Hφ.
+  + term_simpl. constructor.
+    apply jtyping_fmap with (Γ := Γ ↦ₖ tp_cont A).
+    ++ split.
+      - intro x. simpl. apply Hφ.
+      - destruct k as [| k].
+        * simpl. reflexivity.
+        * simpl. apply Hφ.
+    ++ apply H.
+}
+(* jtyping_fmap *)
+{
+  intros Hφ HJ.
+  destruct HJ.
+  + term_simpl. constructor. apply ttyping_fmap with (Γ := Γ).
+    - apply Hφ.
+    - apply H.
+  + econstructor.
+    - apply ktyping_fmap with (Γ := Γ) (q := k_var k).
+      * apply Hφ.
+      * apply H.
+    - apply ttyping_fmap with (Γ := Γ).
+      * apply Hφ.
+      * apply H0.
+}
+Qed.
+
+Lemma ttyping_fmap2 {S T : VSig} (φ : prod_arr S T) (Γ : env S) (Δ : env T) M A :
+  env_map_equiv φ Γ Δ →
+  T[ Δ ⊢ fmap φ M ∷ A ] → T[ Γ ⊢ M ∷ A ]
+with value_fmap2 {S T : VSig} (φ : prod_arr S T) (Γ : env S) (Δ : env T) (V : value S) A :
+  env_map_equiv φ Γ Δ →
+  T[ Δ ⊢ vmap φ V ∷ A ] → T[ Γ ⊢ V ∷ A ]
+with jtyping_fmap2 {S T : VSig} (φ : prod_arr S T) (Γ : env S) (Δ : env T) J :
+  env_map_equiv φ Γ Δ →
+  J[ Δ ⊢ fmap φ J ∷ ⊥⊥ ] → J[ Γ ⊢ J ∷ ⊥⊥ ].
+Proof.
+(* ttyping_fmap2 *)
+{
+  intros Hφ Hfmap.
+  destruct M.
+  + eapply value_fmap2; [ apply Hφ | apply Hfmap ].
+  + inversion Hfmap; subst.
+    econstructor; eauto.
+  + inversion Hfmap; subst.
+    constructor.
+    eapply jtyping_fmap2.
+    * eapply env_map_equiv_kv_extend. apply Hφ.
+    * apply H0.
+}
+(* value_fmap2 *)
+{
+  intros Hφ Hfmap.
+  destruct V.
+  + inversion Hfmap; subst.
+    constructor.
+    rewrite <- (proj1 Hφ). reflexivity.
+  + inversion Hfmap; subst.
+    constructor.
+    eapply ttyping_fmap2.
+    * eapply env_map_equiv_tv_extend. apply Hφ.
+    * apply H0.
+}
+(* jtyping_fmap2 *)
+{
+  intros Hφ Hfmap.
+  destruct J.
+  destruct k.
+  + inversion Hfmap; subst.
+    econstructor.
+    - eapply ktyping_fmap2 with (q := k_var k).
+      * apply Hφ.
+      * apply H1.
+    - eapply ttyping_fmap2.
+      * apply Hφ.
+      * apply H2.
+  + inversion Hfmap; subst.
+    constructor.
+    eapply ttyping_fmap2.
+    * apply Hφ.
+    * apply H0.
+}
+Qed.
+
+Lemma ttyping_tv_weaken {S : VSig} (Γ : env S) M A B :
+  T[ Γ ⊢ M ∷ A ] ↔ T[ Γ ↦ᵥ B ⊢ shift M ∷ A ].
+Proof.
+  split.
+  + apply ttyping_fmap. split; reflexivity.
+  + apply ttyping_fmap2. split; reflexivity.
+Qed.
+
+Lemma ttyping_kv_weaken {S : VSig} (Γ : env S) M A B :
+  T[ Γ ⊢ M ∷ A ] ↔ T[ Γ ↦ₖ B ⊢ shift M ∷ A ].
+Proof.
+  split.
+  + apply ttyping_fmap. split; reflexivity.
+  + apply ttyping_fmap2. split; reflexivity.
+Qed.
+
+Lemma jtyping_kv_weaken {S : VSig} (Γ : env S) J A :
+  J[ Γ ⊢ J ∷ ⊥⊥ ] ↔ J[ Γ ↦ₖ A ⊢ shift J ∷ ⊥⊥ ].
+Proof.
+  split.
+  + apply jtyping_fmap. split; reflexivity.
+  + apply jtyping_fmap2. split; reflexivity.
+Qed.
+
+Lemma jtyping_tv_weaken {S : VSig} (Γ : env S) J A :
+  J[ Γ ⊢ J ∷ ⊥⊥ ] ↔ J[ Γ ↦ᵥ A ⊢ shift J ∷ ⊥⊥ ].
+Proof.
+  split.
+  + apply jtyping_fmap. split; reflexivity.
+  + apply jtyping_fmap2. split; reflexivity.
+Qed.
+
+(* --------------------------------- *)
+
+Lemma etyping_fmap {S T : VSig} (φ : prod_arr S T) (Γ : env S) (Δ : env T) E A B :
+  env_map_equiv φ Γ Δ →
+  E[ Γ ⊢ E ∷ A ⇐ B ] → E[ Δ ⊢ fmap φ E ∷ A ⇐ B ].
+Proof.
+  intros Hφ HE.
+  induction HE.
+  + constructor.
+  + term_simpl. econstructor.
+    - apply IHHE.
+    - apply ttyping_fmap with (Γ := Γ).
+      * apply Hφ.
+      * apply H.
+  + term_simpl. econstructor.
+    - apply ttyping_fmap with (Γ := Γ) (M := V).
+      * apply Hφ.
+      * apply H.
+    - apply IHHE.
+Qed.
+
+Lemma etyping_tv_weaken {S : VSig} (Γ : env S) E A B C :
+  E[ Γ ⊢ E ∷ A ⇐ B ] → E[ Γ ↦ᵥ C ⊢ shift E ∷ A ⇐ B ].
+Proof.
+  apply etyping_fmap. split; reflexivity.
+Qed.
+
+Lemma etyping_kv_weaken {S : VSig} (Γ : env S) E A B C :
+  E[ Γ ⊢ E ∷ A ⇐ B ] → E[ Γ ↦ₖ C ⊢ shift E ∷ A ⇐ B ].
+Proof.
+  apply etyping_fmap. split; reflexivity.
+Qed.
+
+(* ========================================================================= *)
+(* bind, substitution lemmas *)
+
+(* φ is a substitution that preserves types between Γ and Δ. *)
+Definition env_sub_equiv {S T : VSig} (φ : S {→} T) (Γ : env S) (Δ : env T) :=
+  (∀ x, T[ Δ ⊢ sub_v φ x ∷ env_v Γ x ])
+  ∧ (∀ k A B,
+      let (q, E) := sub_k φ k in
+      K[ Γ ⊢ k_var k ∷ A →⊥⊥ ] →
+      K[ Δ ⊢ q ∷ B →⊥⊥ ] →
+      E[ Δ ⊢ E ∷ B ⇐ A ]
+    ).
+
+Lemma env_sub_equiv_tv_extend {S T : VSig} (φ : S {→} T) Γ Δ A :
+  env_sub_equiv φ Γ Δ → env_sub_equiv (φ ↑) (Γ ↦ᵥ A) (Δ ↦ᵥ A).
+Proof.
+  intro Hφ.
+  unfold env_sub_equiv.
+  split.
+  - destruct x as [| x].
+    * simpl. constructor. simpl. reflexivity.
+    * simpl. apply ttyping_tv_weaken with (M := sub_v φ x). apply Hφ.
+  - intros k B C. simpl.
+    destruct (sub_k φ k) as [q E] eqn:Heqsub. simpl.
+    intro Hk.
+
+    destruct Hφ as [Hφᵥ Hφₖ].
+    specialize (Hφₖ k B C). rewrite Heqsub in Hφₖ. rename Hφₖ into HE.
+
+    destruct q as [k' |].
+    * term_simpl. intro Hk'.
+      apply etyping_tv_weaken. apply HE.
+      + eapply ktyping_tv_weaken. apply Hk.
+      + eapply ktyping_tv_weaken. apply Hk'.
+    * term_simpl. intro Htp.
+      apply etyping_tv_weaken. apply HE.
+      + eapply ktyping_tv_weaken. apply Hk.
+      + eapply ktyping_tv_weaken. apply Htp.
+Qed.
+
+Lemma env_sub_equiv_kv_extend {S T : VSig} (φ : S {→} T) Γ Δ A :
+  env_sub_equiv φ Γ Δ → env_sub_equiv (φ ↑) (Γ ↦ₖ A) (Δ ↦ₖ A).
+Proof.
+  intro Hφ.
+  split.
+  - intro x. simpl. apply ttyping_kv_weaken with (M := sub_v φ x). apply Hφ.
+  - intros k B C. simpl.
+    destruct k as [| k].
+    + term_simpl. intros HVZA HVZB.
+      inversion HVZA as [| ? ? HA ]; subst.
+      inversion HVZB as [| ? ? HB ]; subst.
+      simpl in HA, HB. rewrite HA in HB. inversion HB; subst.
+      constructor.
+    + destruct (sub_k φ k) as [q E] eqn:Heqsub. term_simpl.
+      intro Hk.
+
+      destruct Hφ as [Hφᵥ Hφₖ].
+      specialize (Hφₖ k B C). rewrite Heqsub in Hφₖ. rename Hφₖ into HE.
+
+      destruct q as [k' |].
+      * term_simpl. intro Hk'.
+        apply etyping_kv_weaken. apply HE.
+        -- eapply ktyping_kv_weaken. apply Hk.
+        -- eapply ktyping_kv_weaken. apply Hk'.
+      * term_simpl. intro Htp.
+        apply etyping_kv_weaken. apply HE.
+        -- eapply ktyping_kv_weaken. apply Hk.
+        -- eapply ktyping_kv_weaken. apply Htp.
+Qed.
+
+Lemma ttyping_bind {S T : VSig} (φ : S {→} T) (Γ : env S) (Δ : env T) M A :
+  (env_sub_equiv φ Γ Δ) →
+  T[ Γ ⊢ M ∷ A ] → T[ Δ ⊢ bind φ M ∷ A ]
+with jtyping_bind {S T : VSig} (φ : S {→} T) (Γ : env S) (Δ : env T) J :
+  (env_sub_equiv φ Γ Δ) →
+  J[ Γ ⊢ J ∷ ⊥⊥ ] → J[ Δ ⊢ bind φ J ∷ ⊥⊥ ].
+Proof.
+(* ttyping_bind *)
+{
+  intros Hφ HM.
+  generalize dependent Δ.
+  generalize dependent T.
+  induction HM; intros T φ Δ Hφ; unfold bind; term_simpl.
+  + subst. apply Hφ.
+  + econstructor.
+    - apply IHHM1. apply Hφ.
+    - apply IHHM2. apply Hφ.
+  + constructor. apply IHHM.
+    apply env_sub_equiv_tv_extend. apply Hφ.
+  + constructor. apply jtyping_bind with (Γ := Γ ↦ₖ tp_cont A).
+    - apply env_sub_equiv_kv_extend. apply Hφ.
+    - apply H.
+}
+(* jtyping_bind *)
+{
+  intros Hφ HJ.
+  induction HJ; unfold bind; term_simpl.
+  + constructor. apply ttyping_bind with (Γ := Γ).
+    - apply Hφ.
+    - apply H.
+  + destruct (sub_k φ k) as [q E] eqn:Hsub.
+    pose proof Hφ as [Hφᵥ Hφₖ].
+
+    destruct q as [k' |].
+    - destruct (env_k Δ k') as [C] eqn:Heqk'.
+      specialize Hφₖ with k A C. rewrite Hsub in Hφₖ. rename Hφₖ into HE.
+
+      assert (Hk' : K[ Δ ⊢ k_var k' ∷ C →⊥⊥ ]) by (constructor; apply Heqk').
+
+      econstructor.
+      * apply Hk'.
+      * eapply etyping_correct.
+        ++ apply HE.
+          -- apply H.
+          -- apply Hk'.
+        ++ apply ttyping_bind with (Γ := Γ).
+          -- apply Hφ.
+          -- apply H0.
+    - specialize Hφₖ with k A tp_bottom as HE; clear Hφₖ. rewrite Hsub in HE.
+      constructor. eapply etyping_correct.
+      * apply HE.
+        ++ apply H.
+        ++ constructor.
+      * apply ttyping_bind with (Γ := Γ).
+        ++ apply Hφ.
+        ++ apply H0.
+}
+Qed.
+
+Lemma ttyping_subst {S : VSig} (Γ : env S) M (V : value S) A B :
+  T[ Γ ⊢ V ∷ B ] →
+  T[ Γ ↦ᵥ B ⊢ M ∷ A ] →
+  T[ Γ ⊢ subst M V ∷ A ].
+Proof.
+  intros HV HM. unfold subst.
+  apply ttyping_bind with (Γ := Γ ↦ᵥ B).
+  + split.
+    - intro x. simpl.
+      destruct x as [| x].
+      * simpl. apply HV.
+      * simpl. constructor. reflexivity.
+    - intros k C D. simpl.
+      intros HkC HkD. inversion HkC; subst. inversion HkD; subst.
+      simpl in H0. rewrite H0 in H1. inversion H1; subst.
+      constructor.
+  + apply HM.
+Qed.
+
+Lemma jtyping_subst {S : VSig} (Γ : env S) J q E A B :
+  J[ Γ ↦ₖ tp_cont A ⊢ J ∷ ⊥⊥ ] →
+  E[ Γ ⊢ E ∷ B ⇐ A ] →
+  K[ Γ ⊢ q ∷ B →⊥⊥ ] →
+  J[ Γ ⊢ subst J (s_sub q E) ∷ ⊥⊥ ].
+Proof.
+  intros HJ HE Hq.
+  apply jtyping_bind with (Γ := Γ ↦ₖ tp_cont A).
+  + split.
+    - intro x. simpl. constructor. reflexivity.
+    - intros k C D. simpl.
+      destruct k as [| k].
+      * simpl. intro HAC.
+        inversion HAC as [| ? ? HAC']; subst. simpl in HAC'.
+        inversion HAC'; subst; clear HAC'.
+
+        destruct q as [k' |].
+        ++ intro Hk'. inversion Hq as [| ? ? HBk' ]; subst.
+           inversion Hk' as [| ? ? HDk']; subst.
+           rewrite HDk' in HBk'. inversion HBk'; subst.
+           apply HE.
+        ++ intro Htp.
+           inversion Hq; subst.
+           inversion Htp; subst.
+           apply HE.
+      * simpl. intros HCk HDk.
+        inversion HCk as [| ? ? HenvCk]; subst. simpl in HenvCk.
+        inversion HDk as [| ? ? HenvDk]; subst.
+        rewrite HenvCk in HenvDk. inversion HenvDk; subst.
+        constructor.
+  + apply HJ.
+Qed.
+
+Lemma jtyping_struct_subst {S : VSig} (Γ : env S) J E A B :
+  J[ Γ ↦ₖ tp_cont B ⊢ J ∷ ⊥⊥ ] →
+  E[ Γ ↦ₖ tp_cont A ⊢ E ∷ A ⇐ B ] →
+  J[ Γ ↦ₖ tp_cont A ⊢ struct_subst J E ∷ ⊥⊥ ].
+Proof.
+  intros HJ HE.
+  apply jtyping_bind with (Γ := Γ ↦ₖ tp_cont B).
+  + split; term_simpl.
+    - intro x. constructor. reflexivity.
+    - intros k C D. term_simpl.
+      destruct k as [| k].
+      * term_simpl. intros HBC HAD.
+        inversion HBC as [| ? ? HBC']; subst. simpl in HBC'.
+        inversion HAD as [| ? ? HAD']; subst. simpl in HAD'.
+        inversion HBC'; subst; clear HBC'.
+        inversion HAD'; subst; clear HAD'.
+        apply HE.
+      * term_simpl. intros HkC HkD.
+        inversion HkC as [| ? ? HenvkC]; subst. simpl in HenvkC.
+        inversion HkD as [| ? ? HenvkD]; subst. simpl in HenvkD.
+        rewrite HenvkC in HenvkD. inversion HenvkD; subst.
+        constructor.
+  + apply HJ.
+Qed.
