Binding/Env.v
@@ -68,7 +68,7 @@ Proof.
   solve_equiv.
 Qed.
 
-Hint Extern 4 (_ ≡ _) => solve_equiv.
+Hint Extern 4 (_ ≡ _) => solve_equiv : core.
 
 Ltac simpl_HFInd :=
   subst; try discriminate;
