Lang/Preservation.v
@@ -1,0 +1,106 @@
+Require Import Utf8.
+Require Import Syntax Typing Semantics.
+Require Import Binding.Lib Binding.Product.
+
+Lemma tpreservation {S : VSig} : ∀ Γ (M : term S) N A,
+    T[ Γ ⊢ M ∷ A ] →
+    M →ₜ N →
+    T[ Γ ⊢ N ∷ A ]
+with vpreservation {S : VSig} : ∀ Γ (V : value S) V' A,
+    T[ Γ ⊢ V ∷ A ] →
+    V →ᵥ V' →
+    T[ Γ ⊢ V' ∷ A ]
+with jpreservation {S : VSig} : ∀ Γ (J : jump S) J',
+    J[ Γ ⊢ J ∷ ⊥⊥ ] →
+    J →ⱼ J' →
+    J[ Γ ⊢ J' ∷ ⊥⊥ ].
+Proof.
+(* tpreservation *)
+{
+  intros Γ M N A HM Hred.
+  generalize dependent A.
+  induction Hred; intros A HT.
+  + inversion HT as [| ? ? B ? Hlam HV | |]; subst.
+    eapply ttyping_subst.
+    - apply HV.
+    - inversion Hlam as [| | ? ? ? HM |]; subst. apply HM.
+  + inversion HT as [| ? ? B ? Hctrl HN | |]; subst.
+    constructor.
+    eapply jtyping_struct_subst.
+    - inversion Hctrl as [| | | ? ? HJ ]; subst.
+      apply HJ.
+    - econstructor.
+      * constructor.
+      * apply ttyping_kv_weaken. apply HN.
+  + inversion HT as [| ? ? B ? HV Hctrl | |]; subst.
+    constructor.
+    eapply jtyping_struct_subst.
+    - inversion Hctrl as [| | | ? ? HJ ]; subst.
+      apply HJ.
+    - econstructor.
+      * apply ttyping_kv_weaken with (M := V). apply HV.
+      * constructor.
+  + inversion HT as [| | | ? ? Hjmp ]; subst.
+    inversion Hjmp as [| ? B ? HVZ HM ]; subst.
+    simpl in HVZ. inversion HVZ as [| ? ? HAB ]; subst. simpl in HAB.
+    inversion HAB; subst.
+    apply ttyping_kv_weaken in HM.
+    apply HM.
+  + eapply vpreservation.
+    - apply HT.
+    - apply H.
+  + inversion HT as [| ? ? B ? HM HN | |]; subst.
+    econstructor.
+    - eapply tpreservation.
+      * apply HM.
+      * apply Hred.
+    - apply HN.
+  + inversion HT as [| ? ? B ? HM HN | |]; subst.
+    econstructor.
+    - apply HM.
+    - eapply tpreservation.
+      * apply HN.
+      * apply Hred.
+  + inversion HT as [| | | ? ? HJ ]; subst.
+    constructor.
+    eapply jpreservation.
+    - apply HJ.
+    - apply H.
+}
+(* vpreservation *)
+{
+  intros Γ V V' A HT Hred.
+  destruct Hred.
+  + inversion HT as [| | ? B C HM |]; subst.
+    constructor.
+    eapply tpreservation.
+    - apply HM.
+    - apply H.
+}
+(* jpreservation *)
+{
+  intros Γ J J' HT Hred.
+  destruct Hred.
+  + inversion HT as [ ? Hctrl | ? B k Hk Hctrl ]; subst.
+    - inversion Hctrl as [| | | ? ? HJ ]; subst.
+      eapply jtyping_subst.
+      * apply HJ.
+      * constructor.
+      * constructor.
+    - inversion Hctrl as [| | | ? ? HJ ]; subst.
+      eapply jtyping_subst.
+      * apply HJ.
+      * constructor.
+      * apply Hk.
+  + inversion HT as [ ? HM | ? A k Hk HM ]; subst.
+    - constructor.
+      eapply tpreservation.
+      * apply HM.
+      * apply H.
+    - econstructor.
+      * apply Hk.
+      * eapply tpreservation.
+        ++ apply HM.
+        ++ apply H.
+}
+Qed.
