Lang/Semantics.v
@@ -2,6 +2,7 @@ Require Import Utf8.
 Require Import Syntax.
 Require Import Typing.
 Require Import Binding.Lib Binding.Env Binding.Product.
+Require Import Relation_Operators.
 
 Open Scope bind_scope.
 
@@ -9,12 +10,12 @@ Reserved Notation "M '→ₜ' M'" (at level 67).
 Reserved Notation "J '→ⱼ' J'" (at level 67).
 Reserved Notation "V '→ᵥ' V'" (at level 67).
 
-Inductive tred {A : VSig} : term A → term A → Prop :=
-  | tred_beta : ∀ M (V : value A),
+Inductive tred {S : VSig} : term S → term S → Prop :=
+  | tred_beta : ∀ M (V : value S),
     t_app (v_lam M) V →ₜ subst M V
-  | tred_C_L : ∀ (J : jump (incK A)) (N : term A),
+  | tred_C_L : ∀ (J : jump (incK S)) (N : term S),
     t_app (t_ctrl J) N →ₜ t_ctrl (struct_subst J (e_appl e_hole (shift N)))
-  | tred_C_R : ∀ J (V : value A),
+  | tred_C_R : ∀ J (V : value S),
     t_app V (t_ctrl J) →ₜ t_ctrl (struct_subst J (e_appr (shift V) e_hole))
   | tred_C_elim : ∀ M,
     t_ctrl (j_jmp (k_var VZ) (shift M)) →ₜ M
@@ -32,15 +33,15 @@ Inductive tred {A : VSig} : term A → term A → Prop :=
     J →ⱼ J' →
     t_ctrl J →ₜ t_ctrl J'
 
-with jred {A : VSig} : jump A → jump A → Prop :=
-  | jred_idem : ∀ (q : katom (kv A)) (J : jump (incK A)),
+with jred {S : VSig} : jump S → jump S → Prop :=
+  | jred_C_idem : ∀ (q : katom S) (J : jump (incK S)),
     j_jmp q (t_ctrl J) →ⱼ subst J (s_sub q e_hole)
 
   | jred_jmp : ∀ q M M',
     M →ₜ M' →
     j_jmp q M →ⱼ j_jmp q M'
 
-with vred {A : VSig} : value A → value A → Prop :=
+with vred {S : VSig} : value S → value S → Prop :=
   | vred_lam : ∀ M M',
     M →ₜ M' →
     v_lam M →ᵥ v_lam M'
@@ -48,3 +49,11 @@ with vred {A : VSig} : value A → value A → Prop :=
 where "M →ₜ M'" := (tred M M')
   and "J →ⱼ J'" := (jred J J')
   and "V →ᵥ V'" := (vred V V').
+
+Notation tred_rtc M₁ M₂ := (clos_trans_1n _ tred M₁ M₂).
+Notation vred_rtc V₁ V₂ := (clos_trans_1n _ vred V₁ V₂).
+Notation jred_rtc J₁ J₂ := (clos_trans_1n _ jred J₁ J₂).
+
+Notation "M →+ₜ M'" := (tred_rtc M M') (at level 100).
+Notation "J →+ⱼ J'" := (jred_rtc J J') (at level 100).
+Notation "V →+ᵥ V'" := (vred_rtc V V') (at level 100).
